feat(*) shorten reduction compilation 3SAT to IS

HOL_To_IMP/Refinements/HOL_To_IMP_THREE_SAT_To_IS.thy
@@ -1,44 +1,59 @@
 \<^marker>\<open>creator "Kevin Kappelmann"\<close>
 \<^marker>\<open>creator "Nico Lintner"\<close>
+\<^marker>\<open>contributor "Lukas Stevens"\<close>
 theory HOL_To_IMP_THREE_SAT_To_IS
   imports
     HOL_To_IMP_SAT
     Karp21.THREE_SAT_To_IS_List
 begin
 
+paragraph \<open>@{term sat_is_un_1_list}\<close>
+
 context HOL_To_HOL_Nat
-begin       
+begin
 
-lemmas sat_is_un_1_list_fo0_eq = sat_is_un_1_list_fo0_def[unfolded case_prod_unfold]
-function_compile_nat sat_is_un_1_list_fo0_eq
+text \<open>Definitions for higher-order functions passed to @{term list.map}.\<close>
 
-definition "map_acc_sat_is_un_1_list_fo0 i_C l1 \<equiv> map_acc (sat_is_un_1_list_fo0 i_C l1)"
+thm sat_is_un_1_list_def
+
+definition "sat_is_un_1_list_fo0 \<equiv> \<lambda>l1 i l2. if l1 \<noteq> l2 then [[(l1, i), (l2, i)]] else []"
+definition "sat_is_un_1_list_fo1 \<equiv> \<lambda>i C l1. concat (map (sat_is_un_1_list_fo0 l1 i) C)"
+definition "sat_is_un_1_list_fo2 \<equiv> \<lambda>(i, C). concat (map (sat_is_un_1_list_fo1 i C) C)"
+
+lemmas sat_is_un_1_list_fo_defs =
+  sat_is_un_1_list_fo2_def sat_is_un_1_list_fo1_def sat_is_un_1_list_fo0_def
+
+lemma sat_is_un_1_list_fo_def:
+  "sat_is_un_1_list F = concat (map sat_is_un_1_list_fo2 (enumerate 0 F))"
+  unfolding sat_is_un_1_list_fo_defs sat_is_un_1_list_def by simp
+
+function_compile_nat sat_is_un_1_list_fo0_def
+
+definition "map_acc_sat_is_un_1_list_fo0 l1 i \<equiv> map_acc (sat_is_un_1_list_fo0 l1 i)"
 lemmas map_acc_sat_is_un_1_list_fo0_eq =
-  map_acc_eq[of "sat_is_un_1_list_fo0 i_C l1" for i_C l1, folded map_acc_sat_is_un_1_list_fo0_def]  
+  map_acc_eq[of "sat_is_un_1_list_fo0 l1 i" for l1 i, folded map_acc_sat_is_un_1_list_fo0_def]
 function_compile_nat map_acc_sat_is_un_1_list_fo0_eq
 
 lemmas sat_is_un_1_list_fo1_eq =
-  sat_is_un_1_list_fo1_def[unfolded case_prod_unfold map_eq_map_acc_nil,
-    folded map_acc_sat_is_un_1_list_fo0_def]
+  sat_is_un_1_list_fo1_def[unfolded map_eq_map_acc_nil, folded map_acc_sat_is_un_1_list_fo0_def]
 function_compile_nat sat_is_un_1_list_fo1_eq
 
-definition "map_acc_sat_is_un_1_list_fo1 i_C \<equiv> map_acc (sat_is_un_1_list_fo1 i_C)"
+definition "map_acc_sat_is_un_1_list_fo1 i C \<equiv> map_acc (sat_is_un_1_list_fo1 i C)"
 lemmas map_acc_sat_is_un_1_list_fo1_eq =
-  map_acc_eq[of "sat_is_un_1_list_fo1 i_C" for i_C, folded map_acc_sat_is_un_1_list_fo1_def]
+  map_acc_eq[of "sat_is_un_1_list_fo1 i C" for i C, folded map_acc_sat_is_un_1_list_fo1_def]
 function_compile_nat map_acc_sat_is_un_1_list_fo1_eq
 
-lemmas sat_is_un_1_list_fo2_eq =
-  sat_is_un_1_list_fo2_def[unfolded case_prod_unfold map_eq_map_acc_nil,
-    folded map_acc_sat_is_un_1_list_fo1_def]
+lemmas sat_is_un_1_list_fo2_eq = sat_is_un_1_list_fo2_def[
+  unfolded case_prod_unfold map_eq_map_acc_nil, folded map_acc_sat_is_un_1_list_fo1_def]
 function_compile_nat sat_is_un_1_list_fo2_eq
 
-definition "map_acc_sat_is_un_1_list_fo2 \<equiv> map_acc (sat_is_un_1_list_fo2)"
+definition "map_acc_sat_is_un_1_list_fo2 \<equiv> map_acc sat_is_un_1_list_fo2"
 lemmas map_acc_sat_is_un_1_list_fo2_eq =
   map_acc_eq[of "sat_is_un_1_list_fo2", folded map_acc_sat_is_un_1_list_fo2_def]
 function_compile_nat map_acc_sat_is_un_1_list_fo2_eq
 
-lemmas sat_is_un_1_list_fo_eq =
-  sat_is_un_1_list_fo_def[unfolded map_eq_map_acc_nil, folded map_acc_sat_is_un_1_list_fo2_def]
+lemmas sat_is_un_1_list_fo_eq = sat_is_un_1_list_fo_def[
+  unfolded map_eq_map_acc_nil, folded map_acc_sat_is_un_1_list_fo2_def]
 function_compile_nat sat_is_un_1_list_fo_eq
 
 end
@@ -46,52 +61,46 @@ end
 context HOL_Nat_To_IMP
 begin
 
-lemmas sat_is_un_1_list_fo0_nat_eq =
-  HTHN.sat_is_un_1_list_fo0_nat_eq_unfolded[unfolded case_prod_nat_def]
-compile_nat sat_is_un_1_list_fo0_nat_eq
-HOL_To_IMP_correct HOL_To_HOL_Nat.sat_is_un_1_list_fo0_nat
-  by cook
+compile_nat HTHN.sat_is_un_1_list_fo0_nat_eq_unfolded
+HOL_To_IMP_correct HOL_To_HOL_Nat.sat_is_un_1_list_fo0_nat by cook
 
-lemmas map_acc_sat_is_un_1_list_fo0_nat_eq =
-  HTHN.map_acc_sat_is_un_1_list_fo0_nat_eq_unfolded[unfolded case_list_nat_def]
+lemmas map_acc_sat_is_un_1_list_fo0_nat_eq = HTHN.map_acc_sat_is_un_1_list_fo0_nat_eq_unfolded[
+    unfolded case_list_nat_def]
 compile_nat map_acc_sat_is_un_1_list_fo0_nat_eq
 HOL_To_IMP_correct HOL_To_HOL_Nat.map_acc_sat_is_un_1_list_fo0_nat
   apply (tactic \<open>HM.correct_if_IMP_tailcall_correct_tac HT.get_IMP_def @{context} 1\<close>)
-  apply(induction "sat_is_un_1_list_fo0 y ya" _ _ arbitrary: s rule: HTHN.map_acc.induct)
-   apply(cook mode = run_finish)
-  done
+  apply (induction "HTHN.sat_is_un_1_list_fo0 y ya" _ _ arbitrary: s rule: HTHN.map_acc.induct)
+  by (cook mode = run_finish)
 
 compile_nat HTHN.sat_is_un_1_list_fo1_nat_eq_unfolded
-HOL_To_IMP_correct HOL_To_HOL_Nat.sat_is_un_1_list_fo1_nat
-  by cook
+HOL_To_IMP_correct HOL_To_HOL_Nat.sat_is_un_1_list_fo1_nat by cook
 
-lemmas map_acc_sat_is_un_1_list_fo1_nat_eq =
-  HTHN.map_acc_sat_is_un_1_list_fo1_nat_eq_unfolded[unfolded case_list_nat_def]
+lemmas map_acc_sat_is_un_1_list_fo1_nat_eq = HTHN.map_acc_sat_is_un_1_list_fo1_nat_eq_unfolded[
+    unfolded case_list_nat_def]
 compile_nat map_acc_sat_is_un_1_list_fo1_nat_eq
 HOL_To_IMP_correct HOL_To_HOL_Nat.map_acc_sat_is_un_1_list_fo1_nat
   apply (tactic \<open>HM.correct_if_IMP_tailcall_correct_tac HT.get_IMP_def @{context} 1\<close>)
-  apply(induction "sat_is_un_1_list_fo1 y" _ _ arbitrary: s rule: HTHN.map_acc.induct)
-   apply(cook mode = run_finish)
-  done
+  apply (induction "HTHN.sat_is_un_1_list_fo1 y ya" _ _ arbitrary: s rule: HTHN.map_acc.induct)
+  by (cook mode = run_finish)
 
 compile_nat HTHN.sat_is_un_1_list_fo2_nat_eq_unfolded
-HOL_To_IMP_correct HOL_To_HOL_Nat.sat_is_un_1_list_fo2_nat
-  by cook
+HOL_To_IMP_correct HOL_To_HOL_Nat.sat_is_un_1_list_fo2_nat by cook
 
-lemmas map_acc_sat_is_un_1_list_fo2_nat_eq =
-  HTHN.map_acc_sat_is_un_1_list_fo2_nat_eq_unfolded[unfolded case_list_nat_def]
+lemmas map_acc_sat_is_un_1_list_fo2_nat_eq = HTHN.map_acc_sat_is_un_1_list_fo2_nat_eq_unfolded[
+    unfolded case_list_nat_def]
 compile_nat map_acc_sat_is_un_1_list_fo2_nat_eq
 HOL_To_IMP_correct HOL_To_HOL_Nat.map_acc_sat_is_un_1_list_fo2_nat
   apply (tactic \<open>HM.correct_if_IMP_tailcall_correct_tac HT.get_IMP_def @{context} 1\<close>)
-  apply(induction "sat_is_un_1_list_fo2 :: ('a \<times> 'b list) \<Rightarrow> _" _ _ arbitrary: s rule: HTHN.map_acc.induct)
-   apply(cook mode = run_finish)
-  done
+  apply (induction "HTHN.sat_is_un_1_list_fo2 :: ('a \<times> 'b list) \<Rightarrow> _" _ _ arbitrary: s
+    rule: HTHN.map_acc.induct)
+  by (cook mode = run_finish)
 
 compile_nat HTHN.sat_is_un_1_list_nat_eq_unfolded
-HOL_To_IMP_correct HOL_To_HOL_Nat.sat_is_un_1_list_nat
-  by cook
+HOL_To_IMP_correct HOL_To_HOL_Nat.sat_is_un_1_list_nat by cook
 
 end
+
+paragraph \<open>@{term sat_is_un_2_list}\<close>
 
 context HOL_To_HOL_Nat
 begin
@@ -99,38 +108,49 @@ begin
 case_of_simps conflict_lit_eq : conflict_lit.simps
 function_compile_nat conflict_lit_eq
 
-lemmas sat_is_un_2_list_fo0_eq = sat_is_un_2_list_fo0_def[unfolded case_prod_unfold]
-function_compile_nat sat_is_un_2_list_fo0_eq
+thm sat_is_un_2_list_def
 
-definition "map_acc_sat_is_un_2_list_fo0 i_Ci j_Cj l1 \<equiv> map_acc (sat_is_un_2_list_fo0 i_Ci j_Cj l1)"
-lemmas map_acc_sat_is_un_2_list_fo0_eq =                 
-  map_acc_eq[of "sat_is_un_2_list_fo0 i_Ci j_Cj l1" for i_Ci j_Cj l1,
-    folded map_acc_sat_is_un_2_list_fo0_def]  
+definition "sat_is_un_2_list_fo0 \<equiv>
+  \<lambda>l1 i j l2. if conflict_lit l1 l2 then [[(l1, i), (l2, j)]] else []"
+definition "sat_is_un_2_list_fo1 \<equiv> \<lambda>i j Cj l1. concat (map (sat_is_un_2_list_fo0 l1 i j) Cj)"
+definition "sat_is_un_2_list_fo2 \<equiv> \<lambda>i Ci (j, Cj). concat (map (sat_is_un_2_list_fo1 i j Cj) Ci)"
+definition "sat_is_un_2_list_fo3 \<equiv>
+  \<lambda>F (i, Ci). concat (map (sat_is_un_2_list_fo2 i Ci) (enumerate 0 F))"
+
+lemmas sat_is_un_2_list_fo_defs =
+  sat_is_un_2_list_fo0_def sat_is_un_2_list_fo1_def sat_is_un_2_list_fo2_def sat_is_un_2_list_fo3_def
+
+lemma sat_is_un_2_list_fo_def:
+  "sat_is_un_2_list F = concat (map (sat_is_un_2_list_fo3 F) (enumerate 0 F))"
+  unfolding sat_is_un_2_list_def sat_is_un_2_list_fo_defs by simp
+
+function_compile_nat sat_is_un_2_list_fo0_def
+
+definition "map_acc_sat_is_un_2_list_fo0 l1 i j \<equiv> map_acc (sat_is_un_2_list_fo0 l1 i j)"
+lemmas map_acc_sat_is_un_2_list_fo0_eq = map_acc_eq[of "sat_is_un_2_list_fo0 l1 i j" for l1 i j,
+  folded map_acc_sat_is_un_2_list_fo0_def]
 function_compile_nat map_acc_sat_is_un_2_list_fo0_eq
 
-lemmas sat_is_un_2_list_fo1_eq =
-  sat_is_un_2_list_fo1_def[unfolded case_prod_unfold map_eq_map_acc_nil,
-    folded map_acc_sat_is_un_2_list_fo0_def]
+lemmas sat_is_un_2_list_fo1_eq = sat_is_un_2_list_fo1_def[unfolded map_eq_map_acc_nil,
+  folded map_acc_sat_is_un_2_list_fo0_def]
 function_compile_nat sat_is_un_2_list_fo1_eq
 
-definition "map_acc_sat_is_un_2_list_fo1 i_Ci j_Cj \<equiv> map_acc (sat_is_un_2_list_fo1 i_Ci j_Cj)"
+definition "map_acc_sat_is_un_2_list_fo1 i j Cj \<equiv> map_acc (sat_is_un_2_list_fo1 i j Cj)"
 lemmas map_acc_sat_is_un_2_list_fo1_eq =
-  map_acc_eq[of "sat_is_un_2_list_fo1 i_Ci j_Cj" for i_Ci j_Cj, folded map_acc_sat_is_un_2_list_fo1_def]
+  map_acc_eq[of "sat_is_un_2_list_fo1 i j Cj" for i j Cj, folded map_acc_sat_is_un_2_list_fo1_def]
 function_compile_nat map_acc_sat_is_un_2_list_fo1_eq
 
-lemmas sat_is_un_2_list_fo2_eq =
-  sat_is_un_2_list_fo2_def[unfolded case_prod_unfold map_eq_map_acc_nil,
-    folded map_acc_sat_is_un_2_list_fo1_def]
+lemmas sat_is_un_2_list_fo2_eq = sat_is_un_2_list_fo2_def[
+  unfolded case_prod_unfold map_eq_map_acc_nil, folded map_acc_sat_is_un_2_list_fo1_def]
 function_compile_nat sat_is_un_2_list_fo2_eq
 
-definition "map_acc_sat_is_un_2_list_fo2 i_Ci \<equiv> map_acc (sat_is_un_2_list_fo2 i_Ci)"
+definition "map_acc_sat_is_un_2_list_fo2 i Ci \<equiv> map_acc (sat_is_un_2_list_fo2 i Ci)"
 lemmas map_acc_sat_is_un_2_list_fo2_eq =
-  map_acc_eq[of "sat_is_un_2_list_fo2 i_Ci" for i_Ci, folded map_acc_sat_is_un_2_list_fo2_def]
+  map_acc_eq[of "sat_is_un_2_list_fo2 i Ci" for i Ci, folded map_acc_sat_is_un_2_list_fo2_def]
 function_compile_nat map_acc_sat_is_un_2_list_fo2_eq
 
-lemmas sat_is_un_2_list_fo3_eq =
-  sat_is_un_2_list_fo3_def[unfolded case_prod_unfold map_eq_map_acc_nil,
-    folded map_acc_sat_is_un_2_list_fo2_def]
+lemmas sat_is_un_2_list_fo3_eq = sat_is_un_2_list_fo3_def[
+  unfolded case_prod_unfold map_eq_map_acc_nil, folded map_acc_sat_is_un_2_list_fo2_def]
 function_compile_nat sat_is_un_2_list_fo3_eq
 
 definition "map_acc_sat_is_un_2_list_fo3 F \<equiv> map_acc (sat_is_un_2_list_fo3 F)"
@@ -142,7 +162,6 @@ lemmas sat_is_un_2_list_fo_eq =
   sat_is_un_2_list_fo_def[unfolded map_eq_map_acc_nil, folded map_acc_sat_is_un_2_list_fo3_def]
 function_compile_nat sat_is_un_2_list_fo_eq
 
-
 end
 
 context HOL_Nat_To_IMP
@@ -152,63 +171,52 @@ lemmas conflict_lit_nat_eq = HTHN.conflict_lit_nat_eq_unfolded[unfolded case_lit
 compile_nat conflict_lit_nat_eq
 HOL_To_IMP_correct HOL_To_HOL_Nat.conflict_lit_nat by cook
 
-lemmas sat_is_un_2_list_fo0_nat_eq =
-  HTHN.sat_is_un_2_list_fo0_nat_eq_unfolded[unfolded case_prod_nat_def]
-compile_nat sat_is_un_2_list_fo0_nat_eq
-HOL_To_IMP_correct HOL_To_HOL_Nat.sat_is_un_2_list_fo0_nat
-  by cook
+compile_nat HTHN.sat_is_un_2_list_fo0_nat_eq_unfolded
+HOL_To_IMP_correct HOL_To_HOL_Nat.sat_is_un_2_list_fo0_nat by cook
 
 lemmas map_acc_sat_is_un_2_list_fo0_nat_eq =
   HTHN.map_acc_sat_is_un_2_list_fo0_nat_eq_unfolded[unfolded case_list_nat_def]
 compile_nat map_acc_sat_is_un_2_list_fo0_nat_eq
 HOL_To_IMP_correct HOL_To_HOL_Nat.map_acc_sat_is_un_2_list_fo0_nat
   apply (tactic \<open>HM.correct_if_IMP_tailcall_correct_tac HT.get_IMP_def @{context} 1\<close>)
-  apply(induction "sat_is_un_2_list_fo0 y ya yb" _ _ arbitrary: s rule: HTHN.map_acc.induct)
-   apply(cook mode = run_finish)
-  done
+  apply (induction "HTHN.sat_is_un_2_list_fo0 y ya yb" _ _ arbitrary: s rule: HTHN.map_acc.induct)
+  by (cook mode = run_finish)
 
 compile_nat HTHN.sat_is_un_2_list_fo1_nat_eq_unfolded
-HOL_To_IMP_correct HOL_To_HOL_Nat.sat_is_un_2_list_fo1_nat
-  by cook
+HOL_To_IMP_correct HOL_To_HOL_Nat.sat_is_un_2_list_fo1_nat by cook
 
 lemmas map_acc_sat_is_un_2_list_fo1_nat_eq =
   HTHN.map_acc_sat_is_un_2_list_fo1_nat_eq_unfolded[unfolded case_list_nat_def]
 compile_nat map_acc_sat_is_un_2_list_fo1_nat_eq
 HOL_To_IMP_correct HOL_To_HOL_Nat.map_acc_sat_is_un_2_list_fo1_nat
   apply (tactic \<open>HM.correct_if_IMP_tailcall_correct_tac HT.get_IMP_def @{context} 1\<close>)
-  apply(induction "sat_is_un_2_list_fo1 y ya" _ _ arbitrary: s rule: HTHN.map_acc.induct)
-   apply(cook mode = run_finish)
-  done
+  apply (induction "HTHN.sat_is_un_2_list_fo1 y ya yb" _ _ arbitrary: s rule: HTHN.map_acc.induct)
+  by (cook mode = run_finish)
 
 compile_nat HTHN.sat_is_un_2_list_fo2_nat_eq_unfolded
-HOL_To_IMP_correct HOL_To_HOL_Nat.sat_is_un_2_list_fo2_nat
-  by cook
+HOL_To_IMP_correct HOL_To_HOL_Nat.sat_is_un_2_list_fo2_nat by cook
 
 lemmas map_acc_sat_is_un_2_list_fo2_nat_eq =
   HTHN.map_acc_sat_is_un_2_list_fo2_nat_eq_unfolded[unfolded case_list_nat_def]
 compile_nat map_acc_sat_is_un_2_list_fo2_nat_eq
 HOL_To_IMP_correct HOL_To_HOL_Nat.map_acc_sat_is_un_2_list_fo2_nat
   apply (tactic \<open>HM.correct_if_IMP_tailcall_correct_tac HT.get_IMP_def @{context} 1\<close>)
-  apply(induction "sat_is_un_2_list_fo2 y" _ _ arbitrary: s rule: HTHN.map_acc.induct)
-   apply(cook mode = run_finish)
-  done
+  apply (induction "HTHN.sat_is_un_2_list_fo2 y ya" _ _ arbitrary: s rule: HTHN.map_acc.induct)
+  by (cook mode = run_finish)
 
 compile_nat HTHN.sat_is_un_2_list_fo3_nat_eq_unfolded
-HOL_To_IMP_correct HOL_To_HOL_Nat.sat_is_un_2_list_fo3_nat
-  by cook
+HOL_To_IMP_correct HOL_To_HOL_Nat.sat_is_un_2_list_fo3_nat by cook
 
 lemmas map_acc_sat_is_un_2_list_fo3_nat_eq =
   HTHN.map_acc_sat_is_un_2_list_fo3_nat_eq_unfolded[unfolded case_list_nat_def]
 compile_nat map_acc_sat_is_un_2_list_fo3_nat_eq
 HOL_To_IMP_correct HOL_To_HOL_Nat.map_acc_sat_is_un_2_list_fo3_nat
   apply (tactic \<open>HM.correct_if_IMP_tailcall_correct_tac HT.get_IMP_def @{context} 1\<close>)
-  apply(induction "sat_is_un_2_list_fo3 y" _ _ arbitrary: s rule: HTHN.map_acc.induct)
-   apply(cook mode = run_finish)
-  done
+  apply (induction "HTHN.sat_is_un_2_list_fo3 y" _ _ arbitrary: s rule: HTHN.map_acc.induct)
+  by (cook mode = run_finish)
 
 compile_nat HTHN.sat_is_un_2_list_nat_eq_unfolded
-HOL_To_IMP_correct HOL_To_HOL_Nat.sat_is_un_2_list_nat
-  by cook
+HOL_To_IMP_correct HOL_To_HOL_Nat.sat_is_un_2_list_nat by cook
 
 end
 
@@ -232,11 +240,9 @@ corollary sat_is_list_IMP_correct:
     ''sat_is_list_nat.ret'' (natify (sat_is_list x))"
 proof -
   have "Rel_nat (HTHN.sat_is_list_nat TYPE('a) (s ''sat_is_list_nat.arg.x'')) (sat_is_list x)"
-    supply HTHN.sat_is_list_related_transfer[transfer_rule]
-    by transfer_prover
+    supply HTHN.sat_is_list_related_transfer[transfer_rule] by transfer_prover
   then show ?thesis
-    unfolding Rel_nat_iff_eq_natify
-    using sat_is_list_nat_IMP_correct[of s, OF assms] by simp
+    unfolding Rel_nat_iff_eq_natify using sat_is_list_nat_IMP_correct[of s, OF assms] by simp
 qed
 
 end
