Karp21/THREE_SAT_To_IS/THREE_SAT_To_IS_List.thy
@@ -1,5 +1,6 @@
 \<^marker>\<open>creator "Nico Lintner"\<close>
 \<^marker>\<open>contributor "Kevin Kappelmann"\<close>
+\<^marker>\<open>contributor "Lukas Stevens"\<close>
 subsection \<open>Three Sat to Independent Set on Lists\<close>
 theory THREE_SAT_To_IS_List
   imports
@@ -12,79 +13,35 @@ subsubsection \<open>List Definition of @{term sat_is_un_1}\<close>
 definition "sat_is_un_1_list F \<equiv>
   [[(l1, i), (l2, i)]. (i, C) \<leftarrow> enumerate 0 F, l1 \<leftarrow> C, l2 \<leftarrow> C, l1 \<noteq> l2]"
 
-thm sat_is_un_1_list_def
-
-definition "sat_is_un_1_list_fo0 \<equiv>
-  \<lambda>(i, C) l1 l2. if l1 \<noteq> l2 then [[(l1, i), (l2, i)]] else []"
-
-definition "sat_is_un_1_list_fo1 \<equiv>
-  \<lambda>(i, C) l1. concat (map (sat_is_un_1_list_fo0 (i, C) l1) C)"
-
-definition "sat_is_un_1_list_fo2 \<equiv>
-  \<lambda>(i, C). concat (map (sat_is_un_1_list_fo1 (i, C)) C)"
-
-lemmas sat_is_un_1_list_fo_defs =
-  sat_is_un_1_list_fo2_def sat_is_un_1_list_fo1_def sat_is_un_1_list_fo0_def
-
-lemma sat_is_un_1_list_fo_def:
-  "sat_is_un_1_list F = concat (map sat_is_un_1_list_fo2 (enumerate 0 F))"
-  unfolding sat_is_un_1_list_fo_defs sat_is_un_1_list_def
-  by simp
-
-
 text \<open>@{term sat_is_un_1} is related to @{term sat_is_un_1_list}.\<close>
 
 lemma rel_fun_sat_is_un_1_sat_is_un_1_list [transfer_rule]:
   "(list_all2 (Set_List_rel_eq) ===> Set_List_rel Set_List_rel_eq) sat_is_un_1 sat_is_un_1_list"
-  unfolding sat_is_un_1_list_fo_def sat_is_un_1_list_fo_defs sat_is_un_1_def
+  unfolding sat_is_un_1_list_def sat_is_un_1_def
   apply transfer_prover_start
-                      apply transfer_step+
+  apply transfer_step+
   by fastforce
 
- 
 subsubsection \<open>List Definition of @{term sat_is_un_2}\<close>
 
 definition "sat_is_un_2_list F \<equiv>
   [[(l1, i), (l2, j)]. (i, Ci) \<leftarrow> enumerate 0 F, (j, Cj) \<leftarrow> enumerate 0 F,
     l1 \<leftarrow> Ci, l2 \<leftarrow> Cj, conflict_lit l1 l2]"
 
-thm sat_is_un_2_list_def
-
-definition "sat_is_un_2_list_fo0 \<equiv>
-  \<lambda>(i, Ci) (j, Cj) l1 l2. if conflict_lit l1 l2 then [[(l1, i), (l2, j)]] else []"
-
-definition "sat_is_un_2_list_fo1 \<equiv>
-  \<lambda>(i, Ci) (j, Cj) l1. concat (map (sat_is_un_2_list_fo0 (i, Ci) (j, Cj) l1) Cj)"
-
-definition "sat_is_un_2_list_fo2 \<equiv>
-  \<lambda>(i, Ci) (j, Cj). concat (map (sat_is_un_2_list_fo1 (i, Ci) (j, Cj)) Ci)"
-
-definition "sat_is_un_2_list_fo3 \<equiv>
-  \<lambda>F (i, Ci). concat (map (sat_is_un_2_list_fo2 (i, Ci)) (enumerate 0 F))"
-
-lemmas sat_is_un_2_list_fo_defs =
-  sat_is_un_2_list_fo0_def sat_is_un_2_list_fo1_def sat_is_un_2_list_fo2_def sat_is_un_2_list_fo3_def
-
-lemma sat_is_un_2_list_fo_def:
-  "sat_is_un_2_list F = concat (map (sat_is_un_2_list_fo3 F) (enumerate 0 F))"
-  unfolding sat_is_un_2_list_def sat_is_un_2_list_fo_defs by simp
-
-text \<open>Definition equivalent to @{term sat_is_un_2} and closer to @{term sat_is_un_2_list}.\<close>
+text \<open>@{term sat_is_un_2} is related to @{term sat_is_un_2_list}.\<close>
 
 lemma rel_fun_sat_is_un_2_sat_is_un_2_list [transfer_rule]:
   "(list_all2 (Set_List_rel_eq) ===> Set_List_rel Set_List_rel_eq) sat_is_un_2 sat_is_un_2_list"
-  unfolding sat_is_un_2_list_fo_def sat_is_un_2_list_fo_defs sat_is_un_2_def
+  unfolding sat_is_un_2_list_def sat_is_un_2_def
   apply transfer_prover_start
-                      apply transfer_step+
+  apply transfer_step+
   by fastforce
 
 subsubsection \<open>List Definition of @{term sat_is}\<close>
 
-definition
-  "sat_is_list F \<equiv> if is_n_sat_list 3 F
-    then (sat_is_un_1_list F @ sat_is_un_2_list F, length F)
-    else ([], 1)"
-lemmas sat_is_list_unfold = sat_is_list_def[unfolded sat_is_un_1_list_def sat_is_un_2_list_def]
+definition "sat_is_list F \<equiv> if is_n_sat_list 3 F
+  then (sat_is_un_1_list F @ sat_is_un_2_list F, length F)
+  else ([], 1)"
 
 text \<open>@{term sat_is} is related to @{term sat_is_list}.\<close>
 
